concurrency/scache/rwlock/RwLock.i.dfy
@@ -1,0 +1,1588 @@
+include "../../framework/Rw.i.dfy"
+include "../Constants.i.dfy"
+include "FullMap.i.dfy"
+include "CacheHandle.i.dfy"
+include "../../../lib/Base/Option.s.dfy"
+
+module RwLock refines Rw {
+  import opened Constants
+  import opened FullMaps
+  import CacheHandle
+
+  /*
+   * We consider two bits of the status field, ExcLock and Writeback.
+   *
+   * ExcLock and Writeback. Of course, 'ExcLock'
+   * and 'Writeback' should be exclusive operations;
+   * When both flags are set,
+   * it should be interpreted as the 'ExcLock' being
+   * pending, with the 'Writeback' being active.
+   *
+   * Those 2 bits gives 2x2 = 4 states. We then have 2 more:
+   * Unmapped and Reading.
+   *
+   * NOTE: in retrospect, it might have made sense to have this
+   * just be a struct of 5-6 booleans.
+   */
+  datatype Flag =
+    | Unmapped
+    | Reading
+    | Reading_ExcLock
+    | Available
+    | Writeback
+    | Writeback_PendingExcLock
+    | PendingExcLock
+    | ExcLock_Clean
+    | ExcLock_Dirty
+
+  type ThreadId = nat
+
+  type StoredType = CacheHandle.Handle
+
+  // Standard flow for obtaining a 'shared' lock
+
+  datatype SharedState =
+    | SharedPending(t: int)              // inc refcount
+    | SharedPending2(t: int)             // !free & !writelocked
+    | SharedObtained(t: int, b: StoredType)  // !reading
+
+  // Standard flow for obtaining an 'exclusive' lock
+
+  datatype ExcState = 
+    | ExcNone
+      // set ExcLock bit:
+    | ExcPendingAwaitWriteback(t: int, b: StoredType)
+      // check Writeback bit unset
+      //   and `visited` of the refcounts
+    | ExcPending(t: int, visited: int, clean: bool, b: StoredType)
+    | ExcObtained(t: int, clean: bool)
+
+  datatype WritebackState =
+    | WritebackNone
+      // set Writeback status bit
+    | WritebackObtained(b: StoredType)
+
+  // Flow for the phase of reading in a page from disk.
+  // This is a special-case flow, because it needs to be performed
+  // on the way to obtaining a 'shared' lock, but it requires
+  // exclusive access to the underlying memory and resources.
+  // End-game for this flow is to become an ordinary 'shared' lock
+
+  datatype ReadState =
+    | ReadNone
+    | ReadPending                        // set status bit to ExcLock | Reading
+    | ReadPendingCounted(t: ThreadId)    // inc refcount
+    | ReadObtained(t: ThreadId)          // clear ExcLock bit
+
+  datatype CentralState =
+    | CentralNone
+    | CentralState(flag: Flag, stored_value: StoredType)
+
+  datatype M = M(
+    central: CentralState,
+    refCounts: map<ThreadId, nat>,
+
+    ghost sharedState: FullMap<SharedState>,
+    exc: ExcState,
+    read: ReadState,
+
+    // Flow for the phase of doing a write-back.
+    // Special case in part because it can be initiated by any thread
+    // and completed by any thread (not necessarily the same one).
+    
+    writeback: WritebackState
+  ) | Fail
+
+  function unit() : M
+  {
+    M(CentralNone, map[], zero_map(), ExcNone, ReadNone, WritebackNone)
+  }
+
+  function dot(x: M, y: M) : M
+  {
+    if
+      x.M? && y.M?
+      && !(x.central.CentralState? && y.central.CentralState?)
+      && x.refCounts.Keys !! y.refCounts.Keys
+      && (x.exc.ExcNone? || y.exc.ExcNone?)
+      && (x.read.ReadNone? || y.read.ReadNone?)
+      && (x.writeback.WritebackNone? || y.writeback.WritebackNone?)
+    then
+      M(
+        if x.central.CentralState? then x.central else y.central,
+        (map k | k in x.refCounts.Keys + y.refCounts.Keys ::
+            if k in x.refCounts.Keys then x.refCounts[k] else y.refCounts[k]),
+        add_fns(x.sharedState, y.sharedState),
+        if !x.exc.ExcNone? then x.exc else y.exc,
+        if !x.read.ReadNone? then x.read else y.read,
+        if !x.writeback.WritebackNone? then x.writeback else y.writeback
+      ) 
+    else
+      Fail
+  }
+
+  lemma dot_unit(x: M)
+  ensures dot(x, unit()) == x
+  {
+  }
+
+  lemma commutative(x: M, y: M)
+  ensures dot(x, y) == dot(y, x)
+  {
+    if dot(x, y) == Fail {
+      assert dot(x, y) == dot(y, x);
+    } else {
+      assert dot(x, y) == dot(y, x);
+    }
+  }
+
+  lemma associative(x: M, y: M, z: M)
+  ensures dot(x, dot(y, z)) == dot(dot(x, y), z)
+  {
+    assume false;
+  }
+
+  function IsSharedRefFor(t: int) : (SharedState) -> bool
+  {
+    (ss: SharedState) => ss.t == t
+  }
+
+  function CountSharedRefs(m: FullMap<SharedState>, t: int) : nat
+  {
+    SumFilter(IsSharedRefFor(t), m)
+  }
+
+  function CountAllRefs(state: M, t: int) : nat
+  requires state.M?
+  {
+    CountSharedRefs(state.sharedState, t)
+
+      + (if (state.exc.ExcPendingAwaitWriteback?
+            || state.exc.ExcPending?
+            || state.exc.ExcObtained?) && state.exc.t == t
+         then 1 else 0)
+
+      + (if (state.read.ReadPendingCounted?
+            || state.read.ReadObtained?) && state.read.t == t
+         then 1 else 0)
+  }
+
+  predicate Inv(x: M)
+  {
+    && x != unit() ==> (
+      && x.M?
+      && x.central.CentralState?
+      && (x.exc.ExcPendingAwaitWriteback? ==>
+        && x.read.ReadNone?
+        && -1 <= x.exc.t < NUM_THREADS
+        && x.exc.b == x.central.stored_value
+      )
+      && (x.exc.ExcPending? ==>
+        && x.read == ReadNone
+        && x.writeback.WritebackNone?
+        && 0 <= x.exc.visited <= NUM_THREADS
+        && -1 <= x.exc.t < NUM_THREADS
+        && x.exc.b == x.central.stored_value
+      )
+      && (x.exc.ExcObtained? ==>
+        && x.read == ReadNone
+        && x.writeback.WritebackNone?
+        && -1 <= x.exc.t < NUM_THREADS
+      )
+      && (x.writeback.WritebackObtained? ==>
+        && x.read == ReadNone
+        && x.writeback.b == x.central.stored_value
+      )
+      && (x.read.ReadPending? ==>
+        && x.writeback.WritebackNone?
+      )
+      && (x.read.ReadPendingCounted? ==>
+        && x.writeback.WritebackNone?
+        && 0 <= x.read.t < NUM_THREADS
+      )
+      && (x.read.ReadObtained? ==>
+        && 0 <= x.read.t < NUM_THREADS
+      )
+      //&& (x.stored_value.Some? ==>
+      //  x.stored_value.value.is_handle(key)
+      //)
+      && (forall t | 0 <= t < NUM_THREADS
+        :: t in x.refCounts && x.refCounts[t] == CountAllRefs(x, t))
+
+      && (x.central.flag == Unmapped ==>
+        && x.writeback.WritebackNone?
+        && x.read.ReadNone?
+        && x.exc.ExcNone?
+      )
+      && (x.central.flag == Reading ==>
+        && x.read.ReadObtained?
+        && x.writeback.WritebackNone?
+        && x.writeback.WritebackNone?
+      )
+      && (x.central.flag == Reading_ExcLock ==>
+        && (x.read.ReadPending?
+          || x.read.ReadPendingCounted?)
+        && x.writeback.WritebackNone?
+      )
+      && (x.central.flag == Available ==>
+        && x.exc.ExcNone?
+        && x.read.ReadNone?
+        && x.writeback.WritebackNone?
+      )
+      && (x.central.flag == Writeback ==>
+        && x.exc.ExcNone?
+        && x.read.ReadNone?
+        && x.writeback.WritebackObtained?
+      )
+      && (x.central.flag == ExcLock_Clean ==>
+        && (x.exc.ExcPending? || x.exc.ExcObtained?)
+        && x.exc.clean
+        && x.writeback.WritebackNone?
+      )
+      && (x.central.flag == ExcLock_Dirty ==>
+        && (x.exc.ExcPending? || x.exc.ExcObtained?)
+        && !x.exc.clean
+        && x.writeback.WritebackNone?
+      )
+      && (x.central.flag == Writeback_PendingExcLock ==>
+        && x.exc.ExcPendingAwaitWriteback?
+        && x.writeback.WritebackObtained?
+      )
+      && (x.central.flag == PendingExcLock ==>
+        && x.exc.ExcPendingAwaitWriteback?
+        && x.writeback.WritebackNone?
+      )
+      && (forall ss: SharedState :: x.sharedState[ss] > 0 ==>
+        && 0 <= ss.t < NUM_THREADS
+        && (ss.SharedPending2? ==>
+          && !x.exc.ExcObtained?
+          && !x.read.ReadPending?
+          && !x.read.ReadPendingCounted?
+          && (x.exc.ExcPending? ==> x.exc.visited <= ss.t)
+          && x.central.flag != Unmapped
+        )
+        && (ss.SharedObtained? ==>
+          && ss.b == x.central.stored_value
+          && !x.exc.ExcObtained?
+          && x.read.ReadNone?
+          && x.central.flag != Unmapped
+          && (x.exc.ExcPending? ==> x.exc.visited <= ss.t)
+        )
+      )
+    )
+  }
+
+  function I(x: M) : Option<StoredType>
+  //requires Inv(x)
+  {
+    if !x.M? || x == unit() || x.exc.ExcObtained? || !x.read.ReadNone? then (
+      None
+    ) else (
+      Some(x.central.stored_value)
+    )
+  }
+
+  function dot3(a: M, b: M, c: M) : M
+  {
+    dot(dot(a, b), c)
+  }
+
+  ////// Handlers
+
+  function CentralHandle(central: CentralState) : M {
+    M(central, map[], zero_map(), ExcNone, ReadNone, WritebackNone)
+  }
+
+  function RefCount(t: ThreadId, count: nat) : M {
+    M(CentralNone, map[t := count], zero_map(), ExcNone, ReadNone, WritebackNone)
+  }
+
+  function SharedHandle(ss: SharedState) : M {
+    M(CentralNone, map[], unit_fn(ss), ExcNone, ReadNone, WritebackNone)
+  }
+
+  function ReadHandle(r: ReadState) : M {
+    M(CentralNone, map[], zero_map(), ExcNone, r, WritebackNone)
+  }
+
+  function ExcHandle(e: ExcState) : M {
+    M(CentralNone, map[], zero_map(), e, ReadNone, WritebackNone)
+  }
+
+  function WritebackHandle(wb: WritebackState) : M {
+    M(CentralNone, map[], zero_map(), ExcNone, ReadNone, wb)
+  }
+
+  ////// Transitions
+
+  predicate TakeWriteback(m: M, m': M)
+  {
+    && m.M?
+    && m.central.CentralState?
+    && m.central.flag == Available
+
+    && m == CentralHandle(m.central)
+    && m' == dot(
+      CentralHandle(m.central.(flag := Writeback)),
+      WritebackHandle(WritebackObtained(m.central.stored_value))
+    )
+  }
+
+  lemma TakeWriteback_Preserves(m: M, m': M)
+  requires TakeWriteback(m, m')
+  ensures transition(m, m')
+  {
+    forall p: M | Inv(dot(m, p))
+    ensures Inv(dot(m', p)) && I(dot(m, p)) == I(dot(m', p))
+    {
+      assert dot(m', p).sharedState == dot(m, p).sharedState;
+    }
+  }
+
+  predicate ReleaseWriteback(m: M, m': M)
+  {
+    && m.M?
+    && m.central.CentralState?
+    && m.writeback.WritebackObtained?
+
+    && m == dot(
+      CentralHandle(m.central),
+      WritebackHandle(m.writeback)
+    )
+
+    && (m.central.flag == Writeback ==>
+      m' == CentralHandle(m.central.(flag := Available))
+    )
+    && (m.central.flag == Writeback_PendingExcLock ==>
+      m' == CentralHandle(m.central.(flag := PendingExcLock))
+    )
+  }
+
+  lemma ReleaseWriteback_Preserves(m: M, m': M)
+  requires ReleaseWriteback(m, m')
+  ensures transition(m, m')
+  {
+    forall p: M | Inv(dot(m, p))
+    ensures Inv(dot(m', p)) && I(dot(m, p)) == I(dot(m', p))
+    {
+      assert m.central.flag == Writeback
+          || m.central.flag == Writeback_PendingExcLock;
+      assert dot(m', p).sharedState == dot(m, p).sharedState;
+    }
+  }
+
+  predicate ThreadlessExc(m: M, m': M)
+  {
+    && m.M?
+    && m.central.CentralState?
+    && (m.central.flag == Available || m.central.flag == Writeback)
+
+    && m == CentralHandle(m.central)
+    && m' == dot(
+      CentralHandle(m.central.(flag := 
+          if m.central.flag == Available then PendingExcLock else Writeback_PendingExcLock)),
+      ExcHandle(ExcPendingAwaitWriteback(-1, m.central.stored_value))
+    )
+  }
+
+  lemma ThreadlessExc_Preserves(m: M, m': M)
+  requires ThreadlessExc(m, m')
+  ensures transition(m, m')
+  {
+    forall p: M | Inv(dot(m, p))
+    ensures Inv(dot(m', p)) && I(dot(m, p)) == I(dot(m', p))
+    {
+      assert dot(m', p).sharedState == dot(m, p).sharedState;
+    }
+  }
+
+  predicate SharedToExc(m: M, m': M, ss: SharedState)
+  {
+    && m.M?
+    && m.central.CentralState?
+    && (m.central.flag == Available || m.central.flag == Writeback)
+    && ss.SharedObtained?
+
+    && m == dot(
+      CentralHandle(m.central),
+      SharedHandle(ss)
+    )
+    && m' == dot(
+      CentralHandle(m.central.(flag := 
+          if m.central.flag == Available then PendingExcLock else Writeback_PendingExcLock)),
+      ExcHandle(ExcPendingAwaitWriteback(ss.t, ss.b))
+    )
+  }
+
+  lemma SharedToExc_Preserves(m: M, m': M, ss: SharedState)
+  requires SharedToExc(m, m', ss)
+  ensures transition(m, m')
+  {
+    forall p: M | Inv(dot(m, p))
+    ensures Inv(dot(m', p)) && I(dot(m, p)) == I(dot(m', p))
+    {
+      SumFilterSimp<SharedState>();
+
+      assert dot(m', p).refCounts == dot(m, p).refCounts;
+      assert forall b | b != ss :: dot(m', p).sharedState[b] == dot(m, p).sharedState[b];
+      assert dot(m', p).sharedState[ss] + 1 == dot(m, p).sharedState[ss];
+      assert CountAllRefs(dot(m', p), ss.t) == CountAllRefs(dot(m, p), ss.t);
+    }
+  }
+
+  predicate TakeExcLockFinishWriteback(m: M, m': M, clean: bool)
+  {
+    && m.M?
+    && m.central.CentralState?
+    && m.exc.ExcPendingAwaitWriteback?
+    && m.central.flag != Writeback && m.central.flag != Writeback_PendingExcLock
+    && m == dot(
+      CentralHandle(m.central),
+      ExcHandle(m.exc)
+    )
+    && m' == dot(
+      CentralHandle(m.central.(flag :=
+        if clean then ExcLock_Clean else ExcLock_Dirty)),
+      ExcHandle(ExcPending(m.exc.t, 0, clean, m.exc.b))
+    )
+  }
+
+  lemma TakeExcLockFinishWriteback_Preserves(m: M, m': M, clean: bool)
+  requires TakeExcLockFinishWriteback(m, m', clean)
+  ensures transition(m, m')
+  {
+    forall p: M | Inv(dot(m, p))
+    ensures Inv(dot(m', p)) && I(dot(m, p)) == I(dot(m', p))
+    {
+      assert dot(m', p).sharedState == dot(m, p).sharedState;
+    }
+  }
+
+  predicate TakeExcLockCheckRefCount(m: M, m': M)
+  {
+    && m.M?
+    && m.exc.ExcPending?
+    && m.exc.visited in m.refCounts
+    && 0 <= m.exc.visited < NUM_THREADS
+
+    && var expected_rc := (if m.exc.visited == m.exc.t then 1 else 0);
+
+    && m == dot(
+      ExcHandle(m.exc),
+      RefCount(m.exc.visited, expected_rc)
+    )
+    && m' == dot(
+      ExcHandle(m.exc.(visited := m.exc.visited + 1)),
+      RefCount(m.exc.visited, expected_rc)
+    )
+  }
+
+  lemma TakeExcLockCheckRefCount_Preserves(m: M, m': M)
+  requires TakeExcLockCheckRefCount(m, m')
+  ensures transition(m, m')
+  {
+    forall p: M | Inv(dot(m, p))
+    ensures Inv(dot(m', p)) && I(dot(m, p)) == I(dot(m', p))
+    {
+      assert dot(m', p).sharedState == dot(m, p).sharedState;
+      //assert dot(m, p).refCounts[m.exc.visited] == 0;
+      var expected_rc := (if m.exc.visited == m.exc.t then 1 else 0);
+      assert CountAllRefs(dot(m, p), m.exc.visited) == expected_rc;
+      assert CountSharedRefs(dot(m, p).sharedState, m.exc.visited) == 0;
+      UseZeroSum(IsSharedRefFor(m.exc.visited), dot(m, p).sharedState);
+    }
+  }
+
+  predicate Withdraw_TakeExcLockFinish(m: M, m': M, b': StoredType)
+  {
+    && m.M?
+    && m.exc.ExcPending?
+    && m.exc.visited == NUM_THREADS
+    && m == ExcHandle(m.exc)
+    && m' == ExcHandle(ExcObtained(m.exc.t, m.exc.clean))
+    && b' == m.exc.b
+  }
+
+  lemma Withdraw_TakeExcLockFinish_Preserves(m: M, m': M, b': StoredType)
+  requires Withdraw_TakeExcLockFinish(m, m', b')
+  ensures withdraw(m, m', b')
+  {
+    forall p: M | Inv(dot(m, p))
+    ensures Inv(dot(m', p))
+    ensures I(dot(m, p)) == Some(b')
+    ensures I(dot(m', p)) == None
+    {
+      assert dot(m', p).sharedState == dot(m, p).sharedState;
+    }
+  }
+
+  predicate Deposit_DowngradeExcLoc(m: M, m': M, b: StoredType)
+  {
+    && m.M?
+    && m.exc.ExcObtained?
+    && m.central.CentralState?
+    && 0 <= m.exc.t < NUM_THREADS
+    && m == dot(
+      CentralHandle(m.central),
+      ExcHandle(m.exc)
+    )
+    && m' == dot(
+      CentralHandle(m.central
+        .(flag := Available)
+        .(stored_value := b)
+      ),
+      SharedHandle(SharedObtained(m.exc.t, b))
+    )
+  }
+
+  lemma Deposit_DowngradeExcLoc_Preserves(m: M, m': M, b: StoredType)
+  requires Deposit_DowngradeExcLoc(m, m', b)
+  ensures deposit(m, m', b)
+  {
+    forall p: M | Inv(dot(m, p))
+    ensures Inv(dot(m', p))
+    ensures I(dot(m, p)) == None
+    ensures I(dot(m', p)) == Some(b)
+    {
+      SumFilterSimp<SharedState>();
+      var ss := SharedObtained(m.exc.t, b);
+      assert forall b | b != ss :: dot(m', p).sharedState[b] == dot(m, p).sharedState[b];
+      assert dot(m', p).sharedState[ss] == dot(m, p).sharedState[ss] + 1;
+
+      var state' := dot(m', p);
+      forall ss: SharedState | state'.sharedState[ss] > 0
+      ensures 0 <= ss.t < NUM_THREADS
+      ensures (ss.SharedObtained? ==> ss.b == state'.central.stored_value)
+      {
+      }
+    }
+  }
+
+  predicate Withdraw_Alloc(m: M, m': M, b': StoredType)
+  {
+    && m.M?
+    && m.central.CentralState?
+    && m.central.flag == Unmapped
+    && m == CentralHandle(m.central)
+
+    && m' == dot(
+      CentralHandle(m.central.(flag := Reading_ExcLock)),
+      ReadHandle(ReadPending)
+    )
+
+    && b' == m.central.stored_value
+  }
+
+  lemma Withdraw_Alloc_Preserves(m: M, m': M, b': StoredType)
+  requires Withdraw_Alloc(m, m', b')
+  ensures withdraw(m, m', b')
+  {
+    forall p: M | Inv(dot(m, p))
+    ensures Inv(dot(m', p))
+    ensures I(dot(m, p)) == Some(b')
+    ensures I(dot(m', p)) == None
+    {
+      assert dot(m', p).sharedState == dot(m, p).sharedState;
+    }
+  }
+
+  predicate ReadingIncCount(m: M, m': M, t: int)
+  {
+    && m.M?
+    && t in m.refCounts
+    && 0 <= t < NUM_THREADS
+    && m == dot(
+      ReadHandle(ReadPending),
+      RefCount(t, m.refCounts[t])
+    )
+    && m' == dot(
+      ReadHandle(ReadPendingCounted(t)),
+      RefCount(t, m.refCounts[t] + 1)
+    )
+  }
+
+  lemma ReadingIncCount_Preserves(m: M, m': M, t: int)
+  requires ReadingIncCount(m, m', t)
+  ensures transition(m, m')
+  {
+    forall p: M | Inv(dot(m, p))
+    ensures Inv(dot(m', p)) && I(dot(m, p)) == I(dot(m', p))
+    {
+      SumFilterSimp<SharedState>();
+      assert dot(m', p).sharedState == dot(m, p).sharedState;
+      var state := dot(m, p);
+      var state' := dot(m', p);
+      forall t0 | 0 <= t0 < NUM_THREADS
+      ensures t0 in state'.refCounts && state'.refCounts[t0] == CountAllRefs(state', t0)
+      {
+        if t == t0 {
+          assert CountAllRefs(state', t0) == CountAllRefs(state, t0) + 1;
+          assert t0 in state'.refCounts && state'.refCounts[t0] == CountAllRefs(state', t0);
+        } else{
+          assert CountAllRefs(state', t0) == CountAllRefs(state, t0);
+          assert t0 in state'.refCounts && state'.refCounts[t0] == CountAllRefs(state', t0);
+        }
+      }
+    }
+  }
+
+  predicate ObtainReading(m: M, m': M)
+  {
+    && m.M?
+    && m.central.CentralState?
+    && m.read.ReadPendingCounted?
+    && m == dot(
+      CentralHandle(m.central),
+      ReadHandle(m.read)
+    )
+    && m' == dot(
+      CentralHandle(m.central.(flag := Reading)),
+      ReadHandle(ReadObtained(m.read.t))
+    )
+  }
+
+  lemma ObtainReading_Preserves(m: M, m': M)
+  requires ObtainReading(m, m')
+  ensures transition(m, m')
+  {
+    forall p: M | Inv(dot(m, p))
+    ensures Inv(dot(m', p)) && I(dot(m, p)) == I(dot(m', p))
+    {
+    }
+  }
+
+  predicate Deposit_ReadingToShared(m: M, m': M, b: StoredType)
+  {
+    && m.M?
+    && m.central.CentralState?
+    && m.read.ReadObtained?
+    && m == dot(
+      CentralHandle(m.central),
+      ReadHandle(m.read)
+    )
+    && m' == dot(
+      CentralHandle(m.central.(flag := Available).(stored_value := b)),
+      SharedHandle(SharedObtained(m.read.t, b))
+    )
+  }
+
+  lemma Deposit_ReadingToShared_Preserves(m: M, m': M, b: StoredType)
+  requires Deposit_ReadingToShared(m, m', b)
+  ensures deposit(m, m', b)
+  {
+    forall p: M | Inv(dot(m, p))
+    ensures Inv(dot(m', p))
+    ensures I(dot(m, p)) == None
+    ensures I(dot(m', p)) == Some(b)
+    {
+      SumFilterSimp<SharedState>();
+      var state := dot(m, p);
+      var state' := dot(m', p);
+      forall ss: SharedState | state'.sharedState[ss] > 0
+      ensures 0 <= ss.t < NUM_THREADS
+      ensures ss.SharedObtained? ==>
+            && ss.b == state'.central.stored_value
+            && !state'.exc.ExcObtained?
+            && (state'.exc.ExcPending? ==> state'.exc.visited <= ss.t)
+      {
+        if ss.SharedObtained? {
+          assert ss.b == state'.central.stored_value;
+          assert !state'.exc.ExcObtained?;
+          assert (state'.exc.ExcPending? ==> state'.exc.visited <= ss.t);
+        }
+      }
+    }
+  }
+
+  predicate SharedIncCount(m: M, m': M, t: int)
+  {
+    && m.M?
+    && 0 <= t < NUM_THREADS
+    && t in m.refCounts
+    && m == RefCount(t, m.refCounts[t])
+    && m' == dot(
+      RefCount(t, m.refCounts[t] + 1),
+      SharedHandle(SharedPending(t))
+    )
+  }
+
+  lemma SharedIncCount_Preserves(m: M, m': M, t: int)
+  requires SharedIncCount(m, m', t)
+  ensures transition(m, m')
+  {
+    forall p: M | Inv(dot(m, p))
+    ensures Inv(dot(m', p)) && I(dot(m, p)) == I(dot(m', p))
+    {
+      SumFilterSimp<SharedState>();
+      var state := dot(m, p);
+      var state' := dot(m', p);
+      forall t0 | 0 <= t0 < NUM_THREADS
+      ensures t0 in state'.refCounts && state'.refCounts[t0] == CountAllRefs(state', t0)
+      {
+        if t == t0 {
+          assert CountSharedRefs(state.sharedState, t) + 1
+              == CountSharedRefs(state'.sharedState, t);
+          assert CountAllRefs(state, t) + 1
+              == CountAllRefs(state', t);
+          assert t0 in state'.refCounts && state'.refCounts[t0] == CountAllRefs(state', t0);
+        } else {
+          assert CountSharedRefs(state.sharedState, t0) == CountSharedRefs(state'.sharedState, t0);
+          assert CountAllRefs(state, t0) == CountAllRefs(state', t0);
+          assert t0 in state'.refCounts && state'.refCounts[t0] == CountAllRefs(state', t0);
+        }
+      }
+    }
+  }
+
+  predicate SharedDecCountPending(m: M, m': M, t: int)
+  {
+    && m.M?
+    && 0 <= t < NUM_THREADS
+    && t in m.refCounts
+    && m == dot(
+      RefCount(t, m.refCounts[t]),
+      SharedHandle(SharedPending(t))
+    )
+    && (m.refCounts[t] >= 1 ==>
+      m' == RefCount(t, m.refCounts[t] - 1)
+    )
+  }
+
+  lemma SharedDecCountPending_Preserves(m: M, m': M, t: int)
+  requires SharedDecCountPending(m, m', t)
+  ensures transition(m, m')
+  {
+    forall p: M | Inv(dot(m, p))
+    ensures Inv(dot(m', p)) && I(dot(m, p)) == I(dot(m', p))
+    {
+      var state := dot(m, p);
+
+      SumFilterSimp<SharedState>();
+
+      assert state.refCounts[t] >= 1 by {
+        if state.refCounts[t] == 0 {
+          assert CountAllRefs(state, t) == 0;
+          assert CountSharedRefs(state.sharedState, t) == 0;
+          UseZeroSum(IsSharedRefFor(t), state.sharedState);
+          assert false;
+        }
+      }
+
+      var state' := dot(m', p);
+
+      forall t0 | 0 <= t0 < NUM_THREADS
+      ensures t0 in state'.refCounts && state'.refCounts[t0] == CountAllRefs(state', t0)
+      {
+        if t == t0 {
+          assert CountSharedRefs(state.sharedState, t)
+              == CountSharedRefs(state'.sharedState, t) + 1;
+          assert CountAllRefs(state, t)
+              == CountAllRefs(state', t) + 1;
+          assert t0 in state'.refCounts && state'.refCounts[t0] == CountAllRefs(state', t0);
+        } else {
+          assert CountSharedRefs(state.sharedState, t0) == CountSharedRefs(state'.sharedState, t0);
+          assert CountAllRefs(state, t0) == CountAllRefs(state', t0);
+          assert t0 in state'.refCounts && state'.refCounts[t0] == CountAllRefs(state', t0);
+        }
+      }
+    }
+  } 
+
+  predicate SharedDecCountObtained(m: M, m': M, t: int, b: StoredType)
+  {
+    && m.M?
+    && 0 <= t < NUM_THREADS
+    && t in m.refCounts
+    && m == dot(
+      RefCount(t, m.refCounts[t]),
+      SharedHandle(SharedObtained(t, b))
+    )
+    && (m.refCounts[t] >= 1 ==>
+      m' == RefCount(t, m.refCounts[t] - 1)
+    )
+  }
+
+  lemma SharedDecCountObtained_Preserves(m: M, m': M, t: int, b: StoredType)
+  requires SharedDecCountObtained(m, m', t, b)
+  ensures transition(m, m')
+  {
+    forall p: M | Inv(dot(m, p))
+    ensures Inv(dot(m', p)) && I(dot(m, p)) == I(dot(m', p))
+    {
+      var state := dot(m, p);
+
+      SumFilterSimp<SharedState>();
+
+      assert state.refCounts[t] >= 1 by {
+        if state.refCounts[t] == 0 {
+          assert CountAllRefs(state, t) == 0;
+          assert CountSharedRefs(state.sharedState, t) == 0;
+          UseZeroSum(IsSharedRefFor(t), state.sharedState);
+          assert false;
+        }
+      }
+
+      var state' := dot(m', p);
+
+      forall t0 | 0 <= t0 < NUM_THREADS
+      ensures t0 in state'.refCounts && state'.refCounts[t0] == CountAllRefs(state', t0)
+      {
+        if t == t0 {
+          assert CountSharedRefs(state.sharedState, t)
+              == CountSharedRefs(state'.sharedState, t) + 1;
+          assert CountAllRefs(state, t)
+              == CountAllRefs(state', t) + 1;
+          assert t0 in state'.refCounts && state'.refCounts[t0] == CountAllRefs(state', t0);
+        } else {
+          assert CountSharedRefs(state.sharedState, t0) == CountSharedRefs(state'.sharedState, t0);
+          assert CountAllRefs(state, t0) == CountAllRefs(state', t0);
+          assert t0 in state'.refCounts && state'.refCounts[t0] == CountAllRefs(state', t0);
+        }
+      }
+    }
+  } 
+
+  predicate SharedCheckExc(m: M, m': M, t: int)
+  {
+    && m.M?
+    //&& 0 <= t < NUM_THREADS
+    && m.central.CentralState?
+    && (m.central.flag == Available
+        || m.central.flag == Writeback
+        || m.central.flag == Reading)
+    && m == dot(
+      CentralHandle(m.central),
+      SharedHandle(SharedPending(t))
+    )
+    && m' == dot(
+      CentralHandle(m.central),
+      SharedHandle(SharedPending2(t))
+    )
+  }
+
+  lemma SharedCheckExc_Preserves(m: M, m': M, t: int)
+  requires SharedCheckExc(m, m', t)
+  ensures transition(m, m')
+  {
+    forall p: M | Inv(dot(m, p))
+    ensures Inv(dot(m', p)) && I(dot(m, p)) == I(dot(m', p))
+    {
+      SumFilterSimp<SharedState>();
+
+      var state := dot(m, p);
+      var state' := dot(m', p);
+
+      assert CountAllRefs(state, t) == CountAllRefs(state', t);
+      //assert forall t0 | t0 != t :: CountAllRefs(state, t) == CountAllRefs(state', t);
+    }
+  }
+
+  predicate SharedCheckReading(m: M, m': M, t: int)
+  {
+    && m.M?
+    && 0 <= t < NUM_THREADS
+    && m.central.CentralState?
+    && m.central.flag != Reading
+    && m.central.flag != Reading_ExcLock
+    && m == dot(
+      CentralHandle(m.central),
+      SharedHandle(SharedPending2(t))
+    )
+    && m' == dot(
+      CentralHandle(m.central),
+      SharedHandle(SharedObtained(t, m.central.stored_value))
+    )
+  }
+
+  lemma SharedCheckReading_Preserves(m: M, m': M, t: int)
+  requires SharedCheckReading(m, m', t)
+  ensures transition(m, m')
+  {
+    forall p: M | Inv(dot(m, p))
+    ensures Inv(dot(m', p)) && I(dot(m, p)) == I(dot(m', p))
+    {
+      SumFilterSimp<SharedState>();
+
+      var state := dot(m, p);
+      var state' := dot(m', p);
+
+      assert CountAllRefs(state, t) == CountAllRefs(state', t);
+      //assert forall t0 | t0 != t :: CountAllRefs(state, t) == CountAllRefs(state', t);
+    }
+  }
+
+  predicate Deposit_Unmap(m: M, m': M, b: StoredType)
+  {
+    && m.M?
+    && m.exc.ExcObtained?
+    && m.exc.t == -1
+    && m.central.CentralState?
+    && m == dot(
+      CentralHandle(m.central),
+      ExcHandle(m.exc)
+    )
+    && m' == CentralHandle(
+      m.central.(flag := Unmapped).(stored_value := b)
+    )
+  }
+
+  lemma Deposit_Unmap_Preserves(m: M, m': M, b: StoredType)
+  requires Deposit_Unmap(m, m', b)
+  ensures deposit(m, m', b)
+  {
+    forall p: M | Inv(dot(m, p))
+    ensures Inv(dot(m', p))
+    ensures I(dot(m, p)) == None
+    ensures I(dot(m', p)) == Some(b)
+    {
+      assert dot(m', p).sharedState == dot(m, p).sharedState;
+    }
+  }
+
+  predicate AbandonExcPending(m: M, m': M)
+  {
+    && m.M?
+    && m.exc.ExcPending?
+    && m.exc.t == -1
+    && m.central.CentralState?
+    && m == dot(
+      CentralHandle(m.central),
+      ExcHandle(m.exc)
+    )
+    && m' == CentralHandle(m.central.(flag := Available))
+  }
+
+  lemma AbandonExcPending_Preserves(m: M, m': M)
+  requires AbandonExcPending(m, m')
+  ensures transition(m, m')
+  {
+    forall p: M | Inv(dot(m, p))
+    ensures Inv(dot(m', p)) && I(dot(m, p)) == I(dot(m', p))
+    {
+      assert dot(m', p).sharedState == dot(m, p).sharedState;
+    }
+  }
+
+  predicate Deposit_AbandonReadPending(m: M, m': M, b: StoredType)
+  {
+    && m.M?
+    && m.read.ReadPending?
+    && m.central.CentralState?
+    && m == dot(
+      CentralHandle(m.central),
+      ReadHandle(m.read)
+    )
+    && m' == CentralHandle(m.central.(flag := Unmapped).(stored_value := b))
+  }
+
+  lemma Deposit_AbandonReadPending_Preserves(m: M, m': M, b: StoredType)
+  requires Deposit_AbandonReadPending(m, m', b)
+  requires deposit(m, m', b)
+  {
+    forall p: M | Inv(dot(m, p))
+    ensures Inv(dot(m', p))
+    ensures I(dot(m, p)) == None
+    ensures I(dot(m', p)) == Some(b)
+    {
+      assert dot(m', p).sharedState == dot(m, p).sharedState;
+    }
+  }
+}
+
+module RwLockToken {
+  import opened RwLock
+  import opened Constants
+  import opened CacheHandle
+  import T = RwTokens(RwLock)
+
+  type Token = T.Token
+
+  glinear datatype CentralToken = CentralToken(
+    ghost flag: Flag,
+    ghost stored_value: StoredType,
+    glinear token: Token)
+  {
+    predicate has_flag(flag: Flag) {
+      && this.flag == flag
+      && token.val == CentralHandle(CentralState(flag, stored_value))
+    }
+    predicate is_handle(flag: Flag, stored_value: StoredType) {
+      && this.flag == flag
+      && this.stored_value == stored_value
+      && token.val == CentralHandle(CentralState(flag, stored_value))
+    }
+  }
+
+  glinear datatype WritebackObtainedToken = WritebackObtainedToken(
+    ghost b: Handle,
+    glinear token: Token)
+  {
+    predicate has_state(b: StoredType) {
+      && this.b == b
+      && token.val == WritebackHandle(WritebackObtained(b))
+    }
+    predicate is_handle(key: Key) {
+      && b.is_handle(key)
+      && token.val == WritebackHandle(WritebackObtained(b))
+    }
+  }
+
+  glinear datatype SharedPendingToken = SharedToken(
+    ghost t: ThreadId,
+    glinear token: Token)
+  {
+    predicate is_handle(t: ThreadId) {
+      && this.t == t
+      && token.val == SharedHandle(SharedPending(t))
+    }
+  }
+
+  glinear datatype SharedPending2Token = SharedToken(
+    ghost t: ThreadId,
+    glinear token: Token)
+  {
+    predicate is_handle(t: ThreadId) {
+      && this.t == t
+      && token.val == SharedHandle(SharedPending2(t))
+    }
+  }
+
+  glinear datatype SharedObtainedToken = SharedToken(
+    ghost t: ThreadId,
+    ghost b: StoredType,
+    glinear token: Token)
+  {
+    predicate is_handle(t: ThreadId, b: StoredType) {
+      && this.t == t
+      && this.b == b
+      && token.val == SharedHandle(SharedObtained(t, b))
+    }
+  }
+
+  glinear method perform_TakeWriteback(glinear c: Token)
+  returns (glinear c': Token, glinear handle': Token)
+  requires c.val.M?
+  requires var m := c.val;
+    && m.central.CentralState?
+    && m.central.flag == Available
+    && m == CentralHandle(m.central)
+  ensures c'.loc == handle'.loc == c.loc
+  ensures c'.val == CentralHandle(c.val.central.(flag := Writeback))
+  ensures handle'.val == WritebackHandle(WritebackObtained(c.val.central.stored_value))
+  {
+    var a := CentralHandle(c.val.central.(flag := Writeback));
+    var b := WritebackHandle(WritebackObtained(c.val.central.stored_value));
+    TakeWriteback_Preserves(c.val, dot(a, b));
+    c', handle' := T.internal_transition_1_2(c, a, b);
+  }
+
+  glinear method pre_ReleaseWriteback(glinear c: Token, glinear handle: Token)
+  returns (glinear c': Token, glinear handle': Token)
+  requires c.val.M? && handle.val.M?
+  requires var m := c.val;
+    && m.central.CentralState?
+    && m == CentralHandle(m.central)
+  requires var m := handle.val;
+    && m.writeback.WritebackObtained?
+    && m == WritebackHandle(m.writeback)
+  requires c.loc == handle.loc
+  ensures c.val == c'.val && handle'.val == handle.val
+  ensures c.loc == c'.loc && handle'.loc == handle.loc
+  ensures c.val.central.flag == Writeback
+       || c.val.central.flag == Writeback_PendingExcLock
+  {
+    c' := c;
+    handle' := handle;
+    ghost var rest := T.obtain_invariant_2(inout c', inout handle');
+  }
+
+  glinear method perform_ReleaseWriteback(glinear c: Token, glinear handle: Token)
+  returns (glinear c': Token)
+  requires var m := c.val;
+    && m.M?
+    && m.central.CentralState?
+    && m == CentralHandle(m.central)
+  requires var m := handle.val;
+    && m.M?
+    && m.writeback.WritebackObtained?
+    && m == WritebackHandle(m.writeback)
+  requires c.loc == handle.loc
+  ensures c'.loc == c.loc
+  ensures c.val.central.flag == Writeback
+       || c.val.central.flag == Writeback_PendingExcLock
+  ensures c.val.central.flag == Writeback ==>
+      c'.val == CentralHandle(c.val.central.(flag := Available))
+  ensures c.val.central.flag == Writeback_PendingExcLock ==>
+      c'.val == CentralHandle(c.val.central.(flag := PendingExcLock))
+  {
+    var a := CentralHandle(c.val.central.(flag :=
+            if c.val.central.flag == Writeback then Available else PendingExcLock));
+    ReleaseWriteback_Preserves(dot(c.val, handle.val), a);
+    glinear var c1, handle1 := pre_ReleaseWriteback(c, handle);
+    c' := T.internal_transition_2_1(c1, handle1, a);
+  }
+
+  glinear method perform_ThreadlessExc(glinear c: Token)
+  returns (glinear c': Token, glinear handle': Token)
+  requires var m := c.val;
+    && m.M?
+    && m.central.CentralState?
+    && m.central.flag == Available
+    && m == CentralHandle(m.central)
+  ensures c'.loc == handle'.loc == c.loc
+  ensures c'.val == CentralHandle(c.val.central.(flag :=
+      if c.val.central.flag == Available then PendingExcLock else Writeback_PendingExcLock))
+  ensures handle'.val == ExcHandle(ExcPendingAwaitWriteback(-1, c.val.central.stored_value))
+  {
+    var a := CentralHandle(c.val.central.(flag :=
+      if c.val.central.flag == Available then PendingExcLock else Writeback_PendingExcLock));
+    var b := ExcHandle(ExcPendingAwaitWriteback(-1, c.val.central.stored_value));
+    ThreadlessExc_Preserves(c.val, dot(a, b));
+    c', handle' := T.internal_transition_1_2(c, a, b);
+  }
+
+  glinear method perform_SharedToExc(glinear c: Token, glinear handle: Token,
+      ghost ss: SharedState)
+  returns (glinear c': Token, glinear handle': Token)
+  requires ss.SharedObtained?
+  requires var m := c.val;
+    && m.M?
+    && m.central.CentralState?
+    && (m.central.flag == Available || m.central.flag == Writeback)
+    && m == CentralHandle(m.central)
+  requires handle.val == SharedHandle(ss)
+  requires c.loc == handle.loc
+  ensures c'.loc == handle'.loc == c.loc
+  ensures c'.val == CentralHandle(c.val.central.(flag := 
+          if c.val.central.flag == Available then PendingExcLock else Writeback_PendingExcLock))
+  ensures handle'.val == ExcHandle(ExcPendingAwaitWriteback(ss.t, ss.b))
+  {
+    var a := CentralHandle(c.val.central.(flag := 
+          if c.val.central.flag == Available then PendingExcLock else Writeback_PendingExcLock));
+    var b := ExcHandle(ExcPendingAwaitWriteback(ss.t, ss.b));
+    SharedToExc_Preserves(dot(c.val, handle.val), dot(a, b), ss);
+    c', handle' := T.internal_transition_2_2(c, handle, a, b);
+  }
+
+  glinear method perform_TakeExcLockFinishWriteback(glinear c: Token, glinear handle: Token, ghost clean: bool)
+  returns (glinear c': Token, glinear handle': Token)
+  requires var m := c.val;
+    && m.M?
+    && m.central.CentralState?
+    && m.central.flag != Writeback && m.central.flag != Writeback_PendingExcLock
+    && m == CentralHandle(m.central)
+  requires var m := handle.val;
+    && m.M?
+    && m.exc.ExcPendingAwaitWriteback?
+    && m == ExcHandle(m.exc)
+  requires c.loc == handle.loc
+  ensures c.val.central.flag == PendingExcLock
+  ensures c'.loc == handle'.loc == c.loc
+  ensures c'.val == 
+      CentralHandle(c.val.central.(flag :=
+        if clean then ExcLock_Clean else ExcLock_Dirty))
+  ensures handle'.val == 
+      ExcHandle(ExcPending(handle.val.exc.t, 0, clean, handle.val.exc.b))
+  {
+    var a := CentralHandle(c.val.central.(flag :=
+        if clean then ExcLock_Clean else ExcLock_Dirty));
+    var b := ExcHandle(ExcPending(handle.val.exc.t, 0, clean, handle.val.exc.b));
+    TakeExcLockFinishWriteback_Preserves(dot(c.val, handle.val), dot(a, b), clean);
+    c' := c;
+    handle' := handle;
+    var rest := T.obtain_invariant_2(inout c', inout handle');
+    c', handle' := T.internal_transition_2_2(c', handle', a, b);
+  }
+
+  glinear method perform_TakeExcLockCheckRefCount(glinear handle: Token, glinear rc: Token)
+  returns (glinear handle': Token, glinear rc': Token)
+  requires var m := handle.val;
+    && m.M?
+    && m.exc.ExcPending?
+    && m == ExcHandle(m.exc)
+    && 0 <= m.exc.visited < NUM_THREADS
+  requires var expected_rc := (if handle.val.exc.visited == handle.val.exc.t then 1 else 0);
+    && rc.val == RefCount(handle.val.exc.visited, expected_rc)
+  requires rc.loc == handle.loc
+  ensures rc'.loc == handle'.loc == rc.loc
+  ensures handle'.val == ExcHandle(handle.val.exc.(visited := handle.val.exc.visited + 1))
+  ensures rc'.val == rc.val
+  {
+    var a := ExcHandle(handle.val.exc.(visited := handle.val.exc.visited + 1));
+    var b := rc.val;
+    TakeExcLockCheckRefCount_Preserves(dot(handle.val, rc.val), dot(a, b));
+    handle', rc' := T.internal_transition_2_2(handle, rc, a, b);
+  }
+
+  glinear method perform_ReadingIncCount(glinear handle: Token, glinear rc: Token, ghost t: int)
+  returns (glinear handle': Token, glinear rc': Token)
+  requires handle.val == ReadHandle(ReadPending)
+  requires var m := rc.val;
+      && m.M?
+      && t in m.refCounts
+      && 0 <= t < NUM_THREADS
+      && m == RefCount(t, m.refCounts[t])
+  requires handle.loc == rc.loc
+  ensures rc'.loc == handle'.loc == rc.loc
+  ensures handle'.val == ReadHandle(ReadPendingCounted(t))
+  ensures rc'.val == RefCount(t, rc.val.refCounts[t] + 1)
+  {
+    var a := ReadHandle(ReadPendingCounted(t));
+    var b := RefCount(t, rc.val.refCounts[t] + 1);
+    ReadingIncCount_Preserves(dot(handle.val, rc.val), dot(a, b), t);
+    handle', rc' := T.internal_transition_2_2(handle, rc, a, b);
+  }
+
+  glinear method perform_ObtainReading(glinear c: Token, glinear handle: Token)
+  returns (glinear c': Token, glinear handle': Token)
+  requires var m := c.val;
+    && m.M?
+    && m.central.CentralState?
+    && m == CentralHandle(m.central)
+  requires var m := handle.val;
+    && m.M?
+    && m.read.ReadPendingCounted?
+    && m == ReadHandle(m.read)
+  requires c.loc == handle.loc
+  ensures c.val.central.flag == Reading_ExcLock
+  ensures c'.loc == handle'.loc == c.loc
+  ensures c'.val == CentralHandle(c.val.central.(flag := Reading))
+  ensures handle'.val == ReadHandle(ReadObtained(handle.val.read.t))
+  {
+    var a := CentralHandle(c.val.central.(flag := Reading));
+    var b := ReadHandle(ReadObtained(handle.val.read.t));
+    c' := c;
+    handle' := handle;
+    var rest := T.obtain_invariant_2(inout c', inout handle');
+    ObtainReading_Preserves(dot(c.val, handle.val), dot(a, b));
+    c', handle' := T.internal_transition_2_2(c', handle', a, b);
+  }
+
+  glinear method perform_SharedIncCount(glinear rc: Token, ghost t: int)
+  returns (glinear rc': Token, glinear handle': Token)
+  requires var m := rc.val;
+    && m.M?
+    && 0 <= t < NUM_THREADS
+    && t in m.refCounts
+    && m == RefCount(t, m.refCounts[t])
+  ensures rc'.loc == handle'.loc == rc.loc
+  ensures rc'.val == RefCount(t, rc.val.refCounts[t] + 1)
+  ensures handle'.val == SharedHandle(SharedPending(t))
+  {
+    var a := RefCount(t, rc.val.refCounts[t] + 1);
+    var b := SharedHandle(SharedPending(t));
+    SharedIncCount_Preserves(rc.val, dot(a, b), t);
+    rc', handle' := T.internal_transition_1_2(rc, a, b);
+  }
+
+  glinear method pre_SharedDecCountPending(glinear rc: Token, glinear handle: Token, ghost t: int)
+  returns (glinear rc': Token, glinear handle': Token)
+  requires rc.val.M?
+  requires handle.val.M?
+  requires rc.loc == handle.loc
+  requires t in rc.val.refCounts
+  requires handle.val.sharedState[SharedPending(t)] >= 1
+  ensures rc.val.refCounts[t] >= 1
+  ensures handle' == handle
+  ensures rc' == rc
+  {
+    rc' := rc;
+    handle' := handle;
+    ghost var rest := T.obtain_invariant_2(inout rc', inout handle');
+    var m := dot(rc'.val, handle'.val);
+    ghost var state := dot(m, rest);
+    if CountSharedRefs(state.sharedState, t) == 0 {
+      assert state.sharedState[SharedPending(t)] >= 1;
+      FullMaps.UseZeroSum(IsSharedRefFor(t), state.sharedState);
+      assert false;
+    }
+    assert state.refCounts[t] >= 1;
+    assert m.refCounts[t] == state.refCounts[t];
+  }
+
+  glinear method perform_SharedDecCountPending(glinear rc: Token, glinear handle: Token, ghost t: int)
+  returns (glinear rc': Token)
+  requires var m := rc.val;
+    && m.M?
+    && 0 <= t < NUM_THREADS
+    && t in m.refCounts
+    && m == RefCount(t, m.refCounts[t])
+  requires var m := handle.val;
+    && m.M?
+    && m == SharedHandle(SharedPending(t))
+  requires rc.loc == handle.loc
+  ensures rc'.loc == rc.loc
+  ensures rc.val.refCounts[t] >= 1
+  ensures rc'.val == RefCount(t, rc.val.refCounts[t] - 1)
+  {
+    rc' := rc;
+    glinear var handle' := handle;
+    rc', handle' := pre_SharedDecCountPending(rc', handle', t);
+    var a := RefCount(t, rc.val.refCounts[t] - 1);
+    SharedDecCountPending_Preserves(dot(rc'.val, handle.val), a, t);
+    rc' := T.internal_transition_2_1(rc', handle', a);
+  }
+
+  glinear method pre_SharedDecCountObtained(glinear rc: Token, glinear handle: Token, ghost t: int, ghost b: StoredType)
+  returns (glinear rc': Token, glinear handle': Token)
+  requires rc.val.M?
+  requires handle.val.M?
+  requires rc.loc == handle.loc
+  requires t in rc.val.refCounts
+  requires handle.val.sharedState[SharedObtained(t, b)] >= 1
+  ensures rc.val.refCounts[t] >= 1
+  ensures handle' == handle
+  ensures rc' == rc
+  {
+    rc' := rc;
+    handle' := handle;
+    ghost var rest := T.obtain_invariant_2(inout rc', inout handle');
+    var m := dot(rc'.val, handle'.val);
+    ghost var state := dot(m, rest);
+    if CountSharedRefs(state.sharedState, t) == 0 {
+      assert state.sharedState[SharedObtained(t, b)] >= 1;
+      FullMaps.UseZeroSum(IsSharedRefFor(t), state.sharedState);
+      assert false;
+    }
+    assert state.refCounts[t] >= 1;
+    assert m.refCounts[t] == state.refCounts[t];
+  }
+
+  glinear method perform_SharedDecCountObtained(glinear rc: Token, glinear handle: Token,
+      ghost t: int, ghost b: StoredType)
+  returns (glinear rc': Token)
+  requires var m := rc.val;
+    && m.M?
+    && 0 <= t < NUM_THREADS
+    && t in m.refCounts
+    && m == RefCount(t, m.refCounts[t])
+  requires var m := handle.val;
+    && m.M?
+    && m == SharedHandle(SharedObtained(t, b))
+  requires rc.loc == handle.loc
+  ensures rc'.loc == rc.loc
+  ensures rc.val.refCounts[t] >= 1
+  ensures rc'.val == RefCount(t, rc.val.refCounts[t] - 1)
+  {
+    rc' := rc;
+    glinear var handle' := handle;
+    rc', handle' := pre_SharedDecCountObtained(rc', handle', t, b);
+    var a := RefCount(t, rc.val.refCounts[t] - 1);
+    SharedDecCountObtained_Preserves(dot(rc'.val, handle.val), a, t, b);
+    rc' := T.internal_transition_2_1(rc', handle', a);
+  }
+
+  glinear method perform_SharedCheckExc(glinear c: Token, glinear handle: Token, ghost t: int)
+  returns (glinear c': Token, glinear handle': Token)
+  //requires 0 <= t < NUM_THREADS
+  requires var m := c.val;
+    && m.M?
+    && m.central.CentralState?
+    && (m.central.flag == Available
+        || m.central.flag == Writeback
+        || m.central.flag == Reading)
+    && m == CentralHandle(m.central)
+  requires handle.val == SharedHandle(SharedPending(t))
+  requires c.loc == handle.loc
+  ensures c'.loc == handle'.loc == c.loc
+  ensures c'.val == c.val
+  ensures handle'.val == SharedHandle(SharedPending2(t))
+  {
+    var a := c.val;
+    var b := SharedHandle(SharedPending2(t));
+    SharedCheckExc_Preserves(dot(c.val, handle.val), dot(a, b), t);
+    c', handle' := T.internal_transition_2_2(c, handle, a, b);
+  }
+
+  glinear method perform_SharedCheckReading(glinear c: Token, glinear handle: Token, ghost t: int)
+  returns (glinear c': Token, glinear handle': Token)
+  requires 0 <= t < NUM_THREADS
+  requires var m := c.val;
+    && m.M?
+    && m.central.CentralState?
+    && m.central.flag != Reading
+    && m.central.flag != Reading_ExcLock
+    && m == CentralHandle(m.central)
+  requires handle.val == SharedHandle(SharedPending2(t))
+  requires c.loc == handle.loc
+  ensures c'.loc == handle'.loc == c.loc
+  ensures c'.val == c.val
+  ensures handle'.val == SharedHandle(SharedObtained(t, c.val.central.stored_value))
+  {
+    var a := c.val;
+    var b := SharedHandle(SharedObtained(t, c.val.central.stored_value));
+    SharedCheckReading_Preserves(dot(c.val, handle.val), dot(a, b), t);
+    c', handle' := T.internal_transition_2_2(c, handle, a, b);
+  }
+
+  glinear method perform_AbandonExcPending(glinear c: Token, glinear handle: Token)
+  returns (glinear c': Token)
+  requires var m := c.val;
+    && m.M?
+    && m.central.CentralState?
+    && m == CentralHandle(m.central)
+  requires var m := handle.val;
+    && m.M?
+    && m.exc.ExcPending?
+    && m.exc.t == -1
+    && m == ExcHandle(m.exc)
+  requires c.loc == handle.loc
+  ensures c'.loc == c.loc
+  ensures c'.val == CentralHandle(c.val.central.(flag := Available))
+  {
+    var a := CentralHandle(c.val.central.(flag := Available));
+    AbandonExcPending_Preserves(dot(c.val, handle.val), a);
+    c' := T.internal_transition_2_1(c, handle, a);
+  }
+
+  glinear method perform_Withdraw_TakeExcLockFinish(glinear handle: Token)
+  returns (glinear handle': Token, glinear b': Handle)
+  requires var m := handle.val;
+    && m.M?
+    && m.exc.ExcPending?
+    && m.exc.visited == NUM_THREADS
+    && m == ExcHandle(m.exc)
+  ensures handle'.val == ExcHandle(ExcObtained(handle.val.exc.t, handle.val.exc.clean))
+  ensures b' == handle.val.exc.b
+  {
+    var a := ExcHandle(ExcObtained(handle.val.exc.t, handle.val.exc.clean));
+    var d := handle.val.exc.b;
+    Withdraw_TakeExcLockFinish_Preserves(handle.val, a, d);
+    handle', b' := T.withdraw_1_1(handle, a, d);
+  }
+
+  glinear method perform_Withdraw_Alloc(glinear c: Token)
+  returns (glinear c': Token, glinear handle': Token, glinear b': Handle)
+  requires var m := c.val;
+    && m.M?
+    && m.central.CentralState?
+    && m.central.flag == Unmapped
+    && m == CentralHandle(m.central)
+  ensures handle'.loc == c'.loc == c.loc
+  ensures c'.val == CentralHandle(c.val.central.(flag := Reading_ExcLock))
+  ensures handle'.val == ReadHandle(ReadPending)
+  ensures b' == c.val.central.stored_value
+  {
+    var a := CentralHandle(c.val.central.(flag := Reading_ExcLock));
+    var d := ReadHandle(ReadPending);
+    var e := c.val.central.stored_value;
+    Withdraw_Alloc_Preserves(c.val, dot(a, d), e);
+    c', handle', b' := T.withdraw_1_2(c, a, d, e);
+  }
+
+  glinear method perform_Deposit_DowngradeExcLoc(
+      glinear c: Token, glinear handle: Token, glinear b: Handle)
+  returns (glinear c': Token, glinear handle': Token)
+  requires var m := c.val;
+    && m.M?
+    && m.central.CentralState?
+    && m == CentralHandle(m.central)
+  requires var m := handle.val;
+    && m.M?
+    && m.exc.ExcObtained?
+    && 0 <= m.exc.t < NUM_THREADS
+    && m == ExcHandle(m.exc)
+  requires c.loc == handle.loc
+  ensures handle'.loc == c'.loc == c.loc
+  ensures c'.val == 
+      CentralHandle(c.val.central
+        .(flag := Available)
+        .(stored_value := b)
+      )
+  ensures handle'.val ==
+      SharedHandle(SharedObtained(handle.val.exc.t, b))
+  {
+    var a := CentralHandle(c.val.central
+        .(flag := Available)
+        .(stored_value := b)
+      );
+    var d := SharedHandle(SharedObtained(handle.val.exc.t, b));
+    Deposit_DowngradeExcLoc_Preserves(dot(c.val, handle.val), dot(a, d), b);
+    c', handle' := T.deposit_2_2(c, handle, b, a, d);
+  }
+
+  glinear method perform_Deposit_ReadingToShared(
+      glinear c: Token, glinear handle: Token, glinear b: Handle)
+  returns (glinear c': Token, glinear handle': Token)
+  requires var m := c.val;
+    && m.M?
+    && m.central.CentralState?
+    && m == CentralHandle(m.central)
+  requires var m := handle.val;
+    && m.M?
+    && m.read.ReadObtained?
+    && m == ReadHandle(m.read)
+  requires c.loc == handle.loc
+  ensures handle'.loc == c'.loc == c.loc
+  ensures c.val.central.flag == Reading
+  ensures c'.val == 
+      CentralHandle(c.val.central.(flag := Available).(stored_value := b))
+  ensures handle'.val ==
+      SharedHandle(SharedObtained(handle.val.read.t, b))
+  {
+    var a := CentralHandle(c.val.central.(flag := Available).(stored_value := b));
+    var d := SharedHandle(SharedObtained(handle.val.read.t, b));
+    Deposit_ReadingToShared_Preserves(dot(c.val, handle.val), dot(a, d), b);
+    c' := c;
+    handle' := handle;
+    var rest := T.obtain_invariant_2(inout c', inout handle');
+    c', handle' := T.deposit_2_2(c', handle', b, a, d);
+  }
+
+  glinear method perform_Deposit_Unmap(
+      glinear c: Token, glinear handle: Token, glinear b: Handle)
+  returns (glinear c': Token)
+  requires var m := c.val;
+    && m.M?
+    && m.central.CentralState?
+    && m == CentralHandle(m.central)
+  requires var m := handle.val;
+    && m.M?
+    && m.exc.ExcObtained?
+    && m.exc.t == -1
+    && m == ExcHandle(m.exc)
+  requires c.loc == handle.loc
+  ensures c'.loc == c.loc
+  ensures c'.val == 
+    CentralHandle(
+      c.val.central.(flag := Unmapped).(stored_value := b)
+    )
+  {
+    var a := CentralHandle(c.val.central.(flag := Unmapped).(stored_value := b));
+    Deposit_Unmap_Preserves(dot(c.val, handle.val), a, b);
+    c' := T.deposit_2_1(c, handle, b, a);
+  }
+
+  glinear method perform_Deposit_AbandonReadPending(
+      glinear c: Token, glinear handle: Token, glinear b: Handle)
+  returns (glinear c': Token)
+  requires var m := c.val;
+    && m.M?
+    && m.central.CentralState?
+    && m == CentralHandle(m.central)
+  requires var m := handle.val;
+    && m.M?
+    && m.read.ReadPending?
+    && m == ExcHandle(m.exc)
+  requires c.loc == handle.loc
+  ensures c'.loc == c.loc
+  ensures c'.val == 
+    CentralHandle(c.val.central.(flag := Unmapped).(stored_value := b))
+  {
+    var a := CentralHandle(c.val.central.(flag := Unmapped).(stored_value := b));
+    Deposit_AbandonReadPending_Preserves(dot(c.val, handle.val), a, b);
+    c' := T.deposit_2_1(c, handle, b, a);
+  }
+
+/*
+  function method {:opaque} borrow_wb(gshared f: Token) : (gshared b: Handle)
+  requires f.loc.ExtLoc?
+  requires f.loc.base_loc == Base.singleton_loc()
+  requires f.val.writeback.WritebackObtained?
+  ensures b == f.val.writeback.b
+  {
+    ghost var b := Base.one(f.val.writeback.b);
+    Base.unwrap_borrow( borrow_back_interp_exact(f, b) )
+  }
+  */
+}
